Change execution to flater relation structure (Part 1)

src/ReactorModel/Execution/Dependency.lean
@@ -1,6 +1,8 @@
 import ReactorModel.Objects
 
-namespace ReactorType
+open ReactorType
+
+variable [Indexable α]
 
 -- About the `↔`-condition in `prio`:  We want to establish a dependency between mutations with 
 -- priorities as well normal reactions with priorities, but not between normal reactions and
@@ -9,7 +11,7 @@ namespace ReactorType
 -- redundancy.
 --
 -- Note: `Dependency rtr i₁ i₂` means that in `i₁` must occur before `i₂`. 
-inductive Dependency [Indexable α] (rtr : α) : ID → ID → Prop
+inductive Dependency (rtr : α) : ID → ID → Prop
   | prio : 
     (rtr[.rtr][i] = some con) → (con{.rcn}{i₁} = some rcn₁) → (con{.rcn}{i₂} = some rcn₂) → 
     (rcn₁.Mutates ↔ rcn₂.Mutates) → (rcn₁.prio > rcn₂.prio) → Dependency rtr i₁ i₂
@@ -27,54 +29,5 @@ inductive Dependency [Indexable α] (rtr : α) : ID → ID → Prop
 
 notation i₁ " <[" rtr "] " i₂ => Dependency rtr i₁ i₂
 
-namespace Dependency
-
-open Indexable Equivalent
-variable [Indexable α] {rtr rtr₁ : α}
-
-theorem equiv (e : rtr₁ ≈ rtr₂) (d : j₁ <[rtr₂] j₂) : j₁ <[rtr₁] j₂ := by
-  induction d with
-  | prio h₁ h₂ h₃ => 
-    have ⟨_, h₁', e⟩ := Equivalent.obj?_rtr_equiv' e h₁
-    exact prio h₁' (get?_rcn_eq e ▸ h₂) (get?_rcn_eq e ▸ h₃) ‹_› ‹_›
-  | depOverlap h₁ h₂ => 
-    exact depOverlap (e.obj?_rcn_eq.symm ▸ h₁) (e.obj?_rcn_eq.symm ▸ h₂) ‹_› ‹_› ‹_›
-  | mutNorm h₁ h₂ h₃ => 
-    have ⟨_, h₁', e⟩ := Equivalent.obj?_rtr_equiv' e h₁
-    exact mutNorm h₁' (get?_rcn_eq e ▸ h₂) (get?_rcn_eq e ▸ h₃) ‹_› ‹_›
-  | mutNest h₁ h₂ h₃ _ h₄ => 
-    have ⟨_, h₁', e⟩ := Equivalent.obj?_rtr_equiv' e h₁
-    have ⟨_, h₂'⟩ := get?_some_iff e (cpt := .rtr) |>.mpr ⟨_, h₂⟩
-    have h₄' := mem_get?_iff (Equivalent.get?_rtr_some_equiv e h₂' h₂) (cpt := .rcn) |>.mpr h₄
-    exact mutNest h₁' h₂' (get?_rcn_eq e ▸ h₃) ‹_› h₄'
-  | trans _ _ d₁ d₂ => 
-    exact trans d₁ d₂
-
-theorem mem₁ (d : rcn₁ <[rtr] rcn₂) : rcn₁ ∈ rtr[.rcn] := by
-  induction d <;> try exact Partial.mem_iff.mpr ⟨_, obj?_some_extend ‹_› ‹_›⟩ 
-  case depOverlap => exact Partial.mem_iff.mpr ⟨_, ‹_›⟩ 
-  case trans => assumption
-  
-def Acyclic (rtr : α) : Prop :=
+def Dependency.Acyclic (rtr : α) : Prop :=
   ∀ i, ¬(i <[rtr] i)
-
-namespace Acyclic
-
-theorem equiv (e : rtr₁ ≈ rtr₂) (a : Acyclic rtr₁) : Acyclic rtr₂ :=
-  (a · $ ·.equiv e)
-
-theorem iff_mem_acyclic {rtr : α} : (Acyclic rtr) ↔ (∀ i ∈ rtr[.rcn], ¬(i <[rtr] i)) := by
-  apply not_iff_not.mp
-  simp [Acyclic]
-  constructor <;> intro ⟨d, h⟩  
-  case mp  => exact ⟨_, h.mem₁, h⟩
-  case mpr => exact ⟨_, h.right⟩ 
-
-theorem of_trivial (triv : rtr[.rcn] = ∅) : Dependency.Acyclic rtr := by
-  simp_all [Dependency.Acyclic.iff_mem_acyclic, triv]
-  intros _ h
-  exact absurd h Partial.not_mem_empty
-
-end Acyclic
-end Dependency
-end ReactorType
