src/ReactorModel/Execution/Reactor.lean
@@ -1,14 +1,14 @@
 import ReactorModel.Execution.Dependency
-import Mathlib.Data.Finset.Lattice
 
 noncomputable section
 open Classical
 
--- TODO: Split up the following definitions into appropriate namespaces.
 namespace ReactorType
-namespace Practical
 
-variable [Practical α] 
+variable [Indexable α] in section
+
+def dependencies (rtr : α) (rcn : ID) : Set ID := 
+  { rcn' | rcn' <[rtr] rcn }
 
 structure Refresh (rtr₁ rtr₂ : α) (acts : ID ⇀ Value) : Prop where
   equiv    : rtr₁ ≈ rtr₂
@@ -17,36 +17,13 @@ structure Refresh (rtr₁ rtr₂ : α) (acts : ID ⇀ Value) : Prop where
   inputs   : rtr₂[.inp] = rtr₁[.inp].map fun _ => .absent
   outputs  : rtr₂[.out] = rtr₁[.out].map fun _ => .absent
 
-theorem Refresh.deterministic {rtr : α} (rf₁ : Refresh rtr rtr₁ as) (rf₂ : Refresh rtr rtr₂ as) : 
-    rtr₁ = rtr₂ := by
-  have e := Equivalent.trans (Equivalent.symm rf₁.equiv) rf₂.equiv
-  apply Proper.ext_obj? e
-  intro cpt _ _ _ ho₁ ho₂
-  cases cpt
-  case stv => injection (rf₁.eq_state ▸ ho₁) ▸ rf₂.eq_state ▸ ho₂
-  case act => injection (rf₁.acts     ▸ ho₁) ▸ rf₂.acts     ▸ ho₂
-  case inp => injection (rf₁.inputs   ▸ ho₁) ▸ rf₂.inputs   ▸ ho₂
-  case out => injection (rf₁.outputs  ▸ ho₁) ▸ rf₂.outputs  ▸ ho₂
+end
 
-def dependencies (rtr : α) (rcn : ID) : Set ID := 
-  { rcn' | rcn' <[rtr] rcn }
+variable [Proper α] [Finite α]
 
-def dependencies_subset (rtr : α) (rcn : ID) : dependencies rtr rcn ⊆ rtr[.rcn].ids := 
-  fun _ d => d.mem₁
+def refresh (rtr : α) (acts : ID ⇀ Value) : α :=
+  let rtr₁ := set rtr  .inp $ Partial.const (rtr[.inp].ids : Set ID) .absent
+  let rtr₂ := set rtr₁ .out $ Partial.const (rtr[.out].ids : Set ID) .absent
+  set rtr₂ .act acts
 
-theorem equiv_eq_dependencies {rtr₁ : α} (e : rtr₁ ≈ rtr₂) : 
-  dependencies rtr₁ = dependencies rtr₂ := by
-  ext i j
-  exact ⟨.equiv $ .symm e, .equiv e⟩ 
-
-theorem mem_dependencies_subset {rtr : α} {rcn₁ rcn₂ : ID} (h : rcn₂ ∈ dependencies rtr rcn₁) : 
-    dependencies rtr rcn₂ ⊆ dependencies rtr rcn₁ :=
-  fun _ h' => Dependency.trans h' h
-
-theorem mem_dependencies_ssubset {rtr : α} {rcn₁ rcn₂ : ID} 
-    (a : Dependency.Acyclic rtr) (h : rcn₂ ∈ dependencies rtr rcn₁) : 
-    dependencies rtr rcn₂ ⊂ dependencies rtr rcn₁ :=
-  ssubset_iff_subset_ne.mpr ⟨mem_dependencies_subset h, (a _ $ ·.symm ▸ h)⟩
-
-end Practical
 end ReactorType
