src/ReactorModel/Execution/Theorems/Grouped/Instantaneous.lean
@@ -1,11 +1,125 @@
-import ReactorModel.Determinism.InstantaneousStep
+import ReactorModel.Execution.Trace
 
-open Classical
+open ReactorType
 
-namespace Execution
-namespace Instantaneous
-namespace Execution
- 
+namespace Execution.Instantaneous
+
+variable [Indexable α]
+
+inductive Step (s₁ s₂ : State α)
+  | skip (s : s₁ ↓ₛ s₂)
+  | exec (e : s₁ ↓ₑ s₂)
+
+notation s₁:max " ↓ᵢ " s₂:max => Step s₁ s₂
+
+inductive Step.TC : State α → State α → Type
+  | single : (s₁ ↓ᵢ s₂) → TC s₁ s₂
+  | trans  : (s₁ ↓ᵢ s₂) → (TC s₂ s₃) → TC s₁ s₃
+
+notation s₁:max " ↓ᵢ+ " s₂:max => Step.TC s₁ s₂
+
+structure Closed (s₁ s₂ : State α) where
+  exec   : s₁ ↓ᵢ+ s₂ 
+  closed : s₂.Closed
+
+notation s₁:max " ↓ᵢ| " s₂:max => Closed s₁ s₂
+
+/- Step:
+
+variable [Proper α] {s₁ s₂ : State α} in section
+  
+theorem mem_progress_iff (e : s₁ ⇓ᵢ s₂) : rcn' ∈ s₂.progress ↔ rcn' = e.rcn ∨ rcn' ∈ s₁.progress := 
+  by cases e <;> simp [State.mem_record_progress_iff, rcn, State.exec_preserves_progress]
+
+-- Corollary of `InstStep.mem_progress_iff`.
+theorem progress_monotonic (e : s₁ ⇓ᵢ s₂) (h : rcn' ∈ s₁.progress) : rcn' ∈ s₂.progress := 
+  e.mem_progress_iff.mpr $ .inr h
+
+-- Corollary of `InstStep.mem_progress_iff`.
+theorem rcn_mem_progress : (e : s₁ ⇓ᵢ s₂) → e.rcn ∈ s₂.progress := 
+  (·.mem_progress_iff.mpr $ .inl rfl)
+
+theorem rcn_not_mem_progress (e : s₁ ⇓ᵢ s₂) : e.rcn ∉ s₁.progress := 
+  e.allows_rcn.unprocessed
+
+theorem not_closed (e : s₁ ⇓ᵢ s₂) : ¬s₁.Closed :=
+  (· ▸ e.allows_rcn.unprocessed $ e.allows_rcn.mem)
+
+theorem preserves_tag : (s₁ ⇓ᵢ s₂) → s₁.tag = s₂.tag 
+  | skip .. | exec .. => by simp [State.record_preserves_tag, State.exec_preserves_tag]
+
+theorem equiv : (s₁ ⇓ᵢ s₂) → s₁.rtr ≈ s₂.rtr
+  | skip .. => .refl _
+  | exec .. => s₁.exec_equiv _
+
+theorem deterministic (e₁ : s ⇓ᵢ s₁) (e₂ : s ⇓ᵢ s₂) (h : e₁.rcn = e₂.rcn) : s₁ = s₂ := by
+  cases e₁ <;> cases e₂
+  all_goals simp [rcn] at h; subst h; first | rfl | contradiction
+
+theorem acyclic (e : s₁ ⇓ᵢ s₂) : e.rcn ≮[s₁.rtr] e.rcn :=
+  e.allows_rcn.acyclic
+
+theorem progress_eq : (e : s₁ ⇓ᵢ s₂) → s₂.progress = s₁.progress.insert e.rcn
+  | skip .. | exec .. => by simp [State.exec_preserves_progress, State.record]; rfl
+
+theorem progress_ssubset (e : s₁ ⇓ᵢ s₂) : s₁.progress ⊂ s₂.progress := by
+  simp [e.progress_eq, Set.ssubset_iff_insert]
+  exists e.rcn, e.allows_rcn.unprocessed
+
+theorem seq_wellordered (e₁ : s₁ ⇓ᵢ s₂) (e₂ : s₂ ⇓ᵢ s₃) : e₂.rcn ≮[s₁.rtr] e₁.rcn := by
+  by_contra d
+  exact e₂.allows_rcn.unprocessed $ e₁.progress_monotonic $ e₁.allows_rcn.deps d
+
+theorem seq_rcn_ne (e₁ : s₁ ⇓ᵢ s₂) (e₂ : s₂ ⇓ᵢ s₃) : e₁.rcn ≠ e₂.rcn := by
+  by_contra he
+  exact e₂.allows_rcn.unprocessed (he ▸ e₁.rcn_mem_progress)
+
+end
+
+variable [Practical α] {s₁ s₂ s₃ : State α}
+
+theorem prepend_indep' (e₁ : s₁ ⇓ᵢ s₂) (e₂ : s₂ ⇓ᵢ s₃) (h : e₁.rcn ≮[s₁.rtr] e₂.rcn) :
+    ∃ (s₂' : _) (s₃' : _) (e₁' : s₁ ⇓ᵢ s₂') (e₂' : s₂' ⇓ᵢ s₃'), 
+      (e₁'.rcn = e₂.rcn) ∧ (e₂'.rcn = e₁.rcn) ∧ (s₃' = s₃) := by
+  have hi : _ ≮[_]≯ _ := { not_eq := e₁.seq_rcn_ne e₂, left := h, right := e₁.seq_wellordered e₂ }
+  cases e₁ <;> cases e₂ <;> simp [rcn] at hi  
+  case skip.skip ha₁ ht₁ rcn₂ ha₂ ht₂ =>
+    have ha₁' := State.record_indep_allows_iff hi.symm |>.mp ha₁
+    have ha₂' := State.record_indep_allows_iff hi |>.mpr ha₂
+    have ht₁' := State.record_triggers_iff (i₁ := rcn₂) |>.not.mp ht₁
+    have ht₂' := State.record_triggers_iff (i₂ := rcn₂) |>.not.mpr ht₂
+    exact ⟨_, _, Step.skip ha₂' ht₂', Step.skip ha₁' ht₁', rfl, rfl, State.record_comm⟩
+  case skip.exec ha₁ ht₁ _ ha₂ ht₂ =>
+    have ha₁' := State.exec_record_indep_allows_iff hi |>.mp ha₁
+    have ha₂' := State.record_indep_allows_iff hi |>.mpr ha₂
+    have ht₁' := State.exec_record_indep_triggers_iff hi |>.not.mp ht₁
+    have ht₂' := State.record_triggers_iff.mpr ht₂
+    refine ⟨_, _, Step.exec ha₂' ht₂', Step.skip ha₁' ht₁', rfl, rfl, ?_⟩
+    simp [rcn, State.record_exec_comm, State.record_comm]
+  case exec.skip ha₁ ht₁ rcn₂ ha₂ ht₂ => 
+    have ha₁' := State.record_indep_allows_iff hi.symm |>.mp ha₁
+    have ha₂' := State.exec_record_indep_allows_iff hi.symm |>.mpr ha₂
+    have ht₁' := State.record_triggers_iff (i₁ := rcn₂) |>.mp ht₁
+    have ht₂' := State.exec_record_indep_triggers_iff hi.symm |>.not.mpr ht₂
+    refine ⟨_, _, Step.skip ha₂' ht₂', Step.exec ha₁' ht₁', rfl, rfl, ?_⟩
+    simp [rcn, State.record_exec_comm, State.record_comm]
+  case exec.exec ha₁ ht₁ _ ha₂ ht₂ =>
+    have ha₁' := State.exec_record_indep_allows_iff hi |>.mp ha₁
+    have ha₂' := State.exec_record_indep_allows_iff hi.symm |>.mpr ha₂
+    have ht₁' := State.exec_record_indep_triggers_iff hi |>.mp ht₁
+    have ht₂' := State.exec_record_indep_triggers_iff hi.symm |>.mpr ht₂
+    refine ⟨_, _, Step.exec ha₂' ht₂', Step.exec ha₁' ht₁', rfl, rfl, ?_⟩
+    simp [rcn, State.record_exec_comm, State.record_comm, State.exec_indep_comm hi]
+
+theorem prepend_indep (e₁ : s₁ ⇓ᵢ s₂) (e₂ : s₂ ⇓ᵢ s₃) (h : e₁.rcn ≮[s₁.rtr] e₂.rcn) :
+    ∃ (s₂' : _) (e₁' : s₁ ⇓ᵢ s₂') (e₂' : s₂' ⇓ᵢ s₃), (e₁'.rcn = e₂.rcn) ∧ (e₂'.rcn = e₁.rcn) := by
+  have ⟨s₂', _, e₁', e₂', h₁, h₂, h⟩ := prepend_indep' e₁ e₂ h
+  subst h
+  exists s₂', e₁', e₂'
+-/
+
+/- Step.TC:
+
 variable [ReactorType.Practical α] {s₁ s₂ : State α} in section
 
 theorem acyclic (e : s₁ ⇓ᵢ+ s₂) (h : rcn ∈ e.rcns) : rcn ≮[s₁.rtr] rcn := by
@@ -187,7 +301,61 @@ theorem progress_ssubset (e : s₁ ⇓ᵢ+ s₂) : s₁.progress ⊂ s₂.progre
   induction e
   case single e     => exact e.progress_ssubset
   case trans e _ hi => exact e.progress_ssubset |>.trans hi
+-/
 
-end Execution
+/- Closed:
+
+namespace Instantaneous
+namespace ClosedExecution
+
+theorem not_closed (e : s₁ ⇓| s₂) : ¬s₁.Closed := 
+  e.exec.not_closed
+
+theorem nonrepeatable (e₁ : s₁ ⇓| s₂) (e₂ : s₂ ⇓| s₃) : False :=
+  e₂.not_closed e₁.closed
+
+theorem acyclic (e : s₁ ⇓| s₂) (h : rcn ∈ e.rcns) : rcn ≮[s₁.rtr] rcn :=
+  e.exec.acyclic h
+
+theorem preserves_tag (e : s₁ ⇓| s₂) : s₁.tag = s₂.tag :=
+  e.exec.preserves_tag
+
+theorem equiv (e : s₁ ⇓| s₂) : s₁.rtr ≈ s₂.rtr :=
+  e.exec.equiv
+  
+theorem rcns_nodup (e : s₁ ⇓| s₂) : e.rcns.Nodup := 
+  e.exec.rcns_nodup
+
+theorem progress_def (e : s₁ ⇓| s₂) : s₂.progress = s₁.rtr[.rcn].ids :=
+  Equivalent.obj?_rcn_eq e.equiv ▸ e.closed
+
+theorem mem_rcns_iff (e : s₁ ⇓| s₂) : rcn ∈ e.rcns ↔ (rcn ∈ s₁.rtr[.rcn] ∧ rcn ∉ s₁.progress) := by
+  simp [Partial.mem_def, e.progress_def ▸ e.exec.mem_rcns_iff (rcn := rcn)]
+
+theorem progress_empty_mem_rcns_iff (e : s₁ ⇓| s₂) (h : s₁.progress = ∅) : 
+    (rcn ∈ e.rcns) ↔ rcn ∈ s₁.rtr[.rcn] := by
+  simp [e.mem_rcns_iff, h]
+
+theorem rcns_perm (e₁ : s ⇓| s₁) (e₂ : s ⇓| s₂) : e₁.rcns ~ e₂.rcns := by
+  simp [List.perm_ext e₁.rcns_nodup e₂.rcns_nodup, e₁.mem_rcns_iff, e₂.mem_rcns_iff]
+
+theorem tag_eq (e₁ : s ⇓| s₁) (e₂ : s ⇓| s₂) : s₁.tag = s₂.tag :=
+  e₁.exec.preserves_tag ▸ e₂.exec.preserves_tag
+
+theorem progress_eq (e₁ : s ⇓| s₁) (e₂ : s ⇓| s₂) : s₁.progress = s₂.progress := by
+  simp [e₁.progress_def, e₂.progress_def]
+
+theorem step_determined (e : s ⇓| s₁) (a : s ⇓- s₂) : False :=
+  e.not_closed a.closed
+
+theorem progress_ssubset (e : s₁ ⇓| s₂) : s₁.progress ⊂ s₂.progress :=
+  e.exec.progress_ssubset
+
+theorem deterministic (e₁ : s ⇓| s₁) (e₂ : s ⇓| s₂) : s₁ = s₂ :=
+  e₁.exec.deterministic e₂.exec (e₁.tag_eq e₂) (e₁.progress_eq e₂)
+
+end ClosedExecution
 end Instantaneous
-end Execution
+-/
+
+end Execution.Instantaneous
