src/ReactorModel/Execution/Theorems/Nontrivial.lean
@@ -1,10 +1,11 @@
-import ReactorModel.Determinism.ExecutionStep
+import ReactorModel.Execution.Theorems.TimeStep
+import ReactorModel.Execution.Theorems.TimeStep
 
 open ReactorType Classical
 
 namespace Execution
 
-variable [Practical α] {s s₁ s₂ : State α}
+variable [Indexable α] {s s₁ s₂ : State α}
 
 namespace State
 
@@ -20,24 +21,33 @@ theorem Closed.progress_nonempty (n : s.Nontrivial) (h : Closed s) : s.progress.
 
 end State
 
-namespace Advance
-
-theorem preserves_nontrivial {a : s₁ ⇓- s₂} (n : s₁.Nontrivial) : s₂.Nontrivial :=
-  n.equiv a.equiv
-
-theorem not_closed (a : s₁ ⇓- s₂) (n : s₁.Nontrivial) : ¬s₂.Closed :=
-  (·.progress_nonempty (a.preserves_nontrivial n) |>.ne_empty a.progress_empty)
-
-theorem nonrepeatable (a₁ : s₁ ⇓- s₂) (a₂ : s₂ ⇓- s₃) (n : s₁.Nontrivial) : False :=
-  a₁.not_closed n a₂.closed
-
-end Advance
-
-theorem Instantaneous.ClosedExecution.preserves_nontrivial {e : s₁ ⇓| s₂} (n : s₁.Nontrivial) : 
-    s₂.Nontrivial := by
-  simp_all [State.Nontrivial, Equivalent.obj?_rcn_eq e.equiv]
-
 namespace Step
+
+theorem Skip.preserves_nontrivial {e : s₁ ↓ₛ s₂} (n : s₁.Nontrivial) : s₂.Nontrivial :=
+  n.equiv sorry -- e.equiv
+
+theorem Exec.preserves_nontrivial {e : s₁ ↓ₑ s₂} (n : s₁.Nontrivial) : s₂.Nontrivial :=
+  n.equiv sorry -- e.equiv
+
+namespace Time
+
+theorem preserves_nontrivial {e : s₁ ↓ₜ s₂} (n : s₁.Nontrivial) : s₂.Nontrivial :=
+  n.equiv e.equiv
+
+theorem not_closed (e : s₁ ↓ₜ s₂) (n : s₁.Nontrivial) : ¬s₂.Closed :=
+  (·.progress_nonempty (e.preserves_nontrivial n) |>.ne_empty e.progress_empty)
+
+theorem nonrepeatable (e₁ : s₁ ↓ₜ s₂) (e₂ : s₂ ↓ₜ s₃) (n : s₁.Nontrivial) : False :=
+  e₁.not_closed n e₂.closed
+
+end Time
+
+instance preserves_nontrivial (n : s₁.Nontrivial) : (s₁ ↓ s₂) → s₂.Nontrivial
+  | skip e | exec e | time e => e.preserves_nontrivial n
+
+end Step
+
+/-namespace Step
 
 theorem seq_tag_lt (n : s₁.Nontrivial) : (s₁ ⇓ s₂) → (s₂ ⇓ s₃) → s₁.tag < s₃.tag
   | close e₁,   close e₂   => e₁.nonrepeatable e₂ |>.elim
@@ -45,35 +55,33 @@ theorem seq_tag_lt (n : s₁.Nontrivial) : (s₁ ⇓ s₂) → (s₂ ⇓ s₃) �
   | close e,    advance a  => e.preserves_tag ▸ a.tag_lt
   | advance a,  close e    => e.preserves_tag ▸ a.tag_lt
 
-instance preserves_nontrivial (n : s₁.Nontrivial) : (s₁ ⇓ s₂) → s₂.Nontrivial
-  | close e   => e.preserves_nontrivial n
-  | advance a => a.preserves_nontrivial n
-
 end Step
 
 -- TODO: This doesn't require nontrivial.
-theorem tag_le {s₁ s₂ : State α} (e : s₁ ⇓* s₂) : s₁.tag ≤ s₂.tag := by
+theorem tag_le {s₁ s₂ : State α} (e : s₁ ⇓ s₂) : s₁.tag ≤ s₂.tag := by
   induction e with
   | refl        => exact le_refl _
   | step e _ hi => exact le_trans e.tag_le hi
 
 theorem seq_progress_ssubset_or_tag_lt (n : s₁.Nontrivial) : 
-    (s₁ ⇓ s₂) → (s₂ ⇓* s₃) → (s₁.progress ⊂ s₃.progress) ∨ (s₁.tag < s₃.tag)
+    (s₁ ↓ s₂) → (s₂ ⇓ s₃) → (s₁.progress ⊂ s₃.progress) ∨ (s₁.tag < s₃.tag)
   | e₁₂,        step e e' => .inr $ lt_of_lt_of_le (e₁₂.seq_tag_lt n e) e'.tag_le
   | .close e,   refl      => .inl $ e.progress_ssubset
   | .advance a, refl      => .inr $ a.tag_lt
 
 theorem nontrivial_deterministic {s s₁ s₂ : State α} (n : s.Nontrivial)
-    (e₁ : s ⇓* s₁) (e₂ : s ⇓* s₂) (ht : s₁.tag = s₂.tag) (hp : s₁.progress = s₂.progress) : 
+    (e₁ : s ⇓ s₁) (e₂ : s ⇓ s₂) (ht : s₁.tag = s₂.tag) (hp : s₁.progress = s₂.progress) : 
     s₁ = s₂ := by
   induction e₁ generalizing s₂ <;> cases e₂
   case refl.refl => rfl
-  case step.step e₁ _ hi _ e₂ e₂' =>
+  case trans.trans e₁ _ hi _ e₂ e₂' =>
     exact hi (e₁.preserves_nontrivial n) (e₁.deterministic e₂ ▸ e₂') ht hp
   all_goals
-    have e := ‹_ ⇓ _›; have e' := ‹_ ⇓* _›
+    have e := ‹_ ↓  _›; have e' := ‹_ ⇓ _›
     exact match seq_progress_ssubset_or_tag_lt n e e' with
     | .inl h => absurd hp (Set.ssubset_ne $ by simp_all) 
     | .inr h => absurd ht $ ne_of_lt (by simp_all)
+
+-/
 
 end Execution
