src/ReactorModel/Objects/Reactor/Practical.lean
@@ -1,9 +1,0 @@
-import ReactorModel.Objects.Reactor.Finite
-import ReactorModel.Objects.Reactor.Updatable
-import ReactorModel.Objects.Reactor.Proper
-
-namespace ReactorType
-
-class Practical (α) extends Finite α, LawfulUpdatable α, Proper α  
-
-end ReactorType
