src/ReactorModel/Execution/Theorems/Grouped.lean
@@ -1,0 +1,57 @@
+import ReactorModel.Execution.Trace
+import ReactorModel.Execution.Theorems.Grouped.Instantaneous
+import ReactorModel.Execution.Theorems.Grouped.Head
+import ReactorModel.Execution.Theorems.Grouped.Steps
+import ReactorModel.Execution.Theorems.Grouped.Tail
+import ReactorModel.Execution.Theorems.Nontrivial
+
+open ReactorType
+
+namespace Execution
+
+structure Grouped [Indexable α] (s₁ s₂ : State α) where
+  hd    : State α
+  tl    : State α
+  head  : Grouped.Head  s₁ hd
+  steps : Grouped.Steps hd tl
+  tail  : Grouped.Tail  tl s₂
+
+-- TODO: You can add a condition of nontriviality if you want.
+--       In fact, the theorems in Nontrivial.lean are probably the right ones to solve this.
+theorem Grouped.deterministic 
+    [Proper α] {s s₁ s₂ : State α} (ht : s₁.tag = s₂.tag) (hp : s₁.progress = s₂.progress) :
+    (Grouped s s₁) → (Grouped s s₂) → s₁ = s₂ := by
+  intro ⟨hd₁, tl₁, head₁, steps₁, tail₁⟩ ⟨hd₂, tl₂, head₂, steps₂, tail₂⟩
+  /-replace ht : tl₁.tag = tl₂.tag := tail₁.preserves_tag ▸ tail₂.preserves_tag ▸ ht
+  suffices h : hd₁ = hd₂ by
+    subst h
+    cases steps₁.deterministic steps₂ ht
+    cases tail₁.deterministic tail₂ hp
+    rfl
+  -/
+  sorry 
+
+-- TODO: Move this theorem into the Nontrivial.lean file?
+def grouped [Indexable α] : {s₁ s₂ : State α} → (n : s₁.Nontrivial) → (s₁ ⇓ s₂) → Grouped s₁ s₂
+  | s, _, _, .refl => 
+    ⟨s, s, .nil, .refl, .nil⟩ 
+  | s₁, s₃, n, .trans (.skip e) e' (s₂ := s₂) => 
+    let ⟨hd, tl, head, steps, tail⟩ := e'.grouped $ e.preserves_nontrivial n
+    match hh : head, hs : steps, ht : tail with
+    | .nil,    .refl,    .nil    => sorry -- contradiction by e
+    | .nil,    .refl,    .time _ => sorry -- ⟨s₁, s₁, .nil, .refl, .inst $ .trans (.skip e) f⟩
+    | .nil,    .step .., .nil    => sorry
+    | .nil,    .step .., .time _ => sorry
+    | .inst _, .refl,    .nil    => sorry
+    | .inst _, .refl,    .time _ => sorry
+    | .inst _, .step .., .nil    => sorry
+    | .inst _, .step .., .time _ => sorry
+  | s₁, s₂, _, .trans (.exec e) e' => sorry -- this should be identical to the one above
+  | s₁, s₃, n, .trans (.time e) e' (s₂ := s₂) => 
+    let g := e'.grouped $ e.preserves_nontrivial n
+    sorry
+    -- match h : g.head with
+    -- | .nil    => { g with head := .time $ (symm ‹_› : s₂ = g.hd) ▸ e }
+    -- | .time f => e.nonrepeatable f n |>.elim
+
+end Execution
