src/ReactorModel/Execution/Theorems/Grouped/Steps.lean
@@ -1,0 +1,23 @@
+import ReactorModel.Execution.Trace
+import ReactorModel.Execution.Theorems.Grouped.Instantaneous
+
+open ReactorType
+
+namespace Execution.Grouped
+
+variable [Indexable α]
+
+inductive Steps : State α → State α → Type 
+  | refl : Steps s s
+  | step : (s₂ ↓ₜ s₃) → (s₁ ↓ᵢ| s₂) → (Steps s₃ s₄) → Steps s₁ s₄ 
+
+namespace Steps
+
+theorem tag_strictly_monotonic {s₁ : State α} (e : Steps s₁ s₂) : s₁.tag < s₂.tag := by
+  sorry
+
+theorem deterministic {s₁ s₂ : State α} (e₁ : Steps s s₁) (e₂ : Steps s s₂) 
+    (ht : s₁.tag = s₂.tag) : s₁ = s₂ := by
+  sorry
+
+end Execution.Grouped.Steps
