src/ReactorModel/Execution/Theorems/Grouped/Tail.lean
@@ -1,0 +1,12 @@
+import ReactorModel.Execution.Trace
+open ReactorType
+
+namespace Execution.Grouped
+
+variable [Indexable α]
+
+inductive Tail : State α → State α → Type
+  | nil  : Tail s s
+  | time : (s₁ ↓ₜ s₂) → Tail s₁ s₂
+
+end Execution.Grouped
