src/ReactorModel/Execution/Theorems/Reactor.lean
@@ -1,0 +1,64 @@
+import ReactorModel.Execution.Reactor
+import ReactorModel.Execution.Theorems.Dependency
+
+namespace ReactorType
+
+variable [Indexable α] in section
+
+theorem dependencies_subset (rtr : α) (rcn : ID) : dependencies rtr rcn ⊆ rtr[.rcn].ids := 
+  fun _ d => d.mem₁
+
+theorem equiv_eq_dependencies {rtr₁ : α} (e : rtr₁ ≈ rtr₂) : 
+  dependencies rtr₁ = dependencies rtr₂ := by
+  ext i j
+  exact ⟨.equiv $ .symm e, .equiv e⟩ 
+
+theorem mem_dependencies_subset {rtr : α} {rcn₁ rcn₂ : ID} (h : rcn₂ ∈ dependencies rtr rcn₁) : 
+    dependencies rtr rcn₂ ⊆ dependencies rtr rcn₁ :=
+  fun _ h' => Dependency.trans h' h
+
+theorem mem_dependencies_ssubset {rtr : α} {rcn₁ rcn₂ : ID} 
+    (a : Dependency.Acyclic rtr) (h : rcn₂ ∈ dependencies rtr rcn₁) : 
+    dependencies rtr rcn₂ ⊂ dependencies rtr rcn₁ :=
+  ssubset_iff_subset_ne.mpr ⟨mem_dependencies_subset h, (a _ $ ·.symm ▸ h)⟩
+
+end
+
+variable [Proper α]
+
+theorem Refresh.deterministic {rtr : α} (rf₁ : Refresh rtr rtr₁ as) (rf₂ : Refresh rtr rtr₂ as) : 
+    rtr₁ = rtr₂ := by
+  have e := Equivalent.trans (Equivalent.symm rf₁.equiv) rf₂.equiv
+  apply ext_obj? e
+  intro cpt _ _ _ ho₁ ho₂
+  cases cpt
+  case stv => injection (rf₁.eq_state ▸ ho₁) ▸ rf₂.eq_state ▸ ho₂
+  case act => injection (rf₁.acts     ▸ ho₁) ▸ rf₂.acts     ▸ ho₂
+  case inp => injection (rf₁.inputs   ▸ ho₁) ▸ rf₂.inputs   ▸ ho₂
+  case out => injection (rf₁.outputs  ▸ ho₁) ▸ rf₂.outputs  ▸ ho₂
+
+variable [Finite α]
+
+theorem refresh_correct (rtr : α) (h : acts.ids = rtr[.act].ids) : 
+    Refresh rtr (refresh rtr acts) acts where
+  equiv := Equivalent.trans set_equiv $ Equivalent.trans set_equiv set_equiv
+  eq_state := by
+    rw [
+      refresh, set_preserves (by simp : .stv ≠ .act), set_preserves (by simp : .stv ≠ .out), 
+      set_preserves (by simp : .stv ≠ .inp)
+    ]
+  acts := by 
+    rw [refresh, set_updated' $ h ▸ (Equivalent.ids_eq $ Equivalent.trans set_equiv set_equiv)]
+  inputs := by 
+    rw [
+      refresh, set_preserves (by simp : .inp ≠ .act), set_preserves (by simp : .inp ≠ .out), 
+      set_updated' $ Partial.const_ids _ _, Partial.const_eq_map_const
+    ]
+  outputs := by 
+    rw [
+      refresh, set_preserves (by simp : .out ≠ .act),
+      set_updated' $ by rw [Equivalent.ids_eq set_equiv, Partial.const_ids _ _],
+      Partial.const_eq_map_const
+    ]
+
+end ReactorType
