src/ReactorModel/Objects/Reactor.lean
@@ -2,7 +2,6 @@ import ReactorModel.Objects.Reactor.Basic
 import ReactorModel.Objects.Reactor.Extensional
 import ReactorModel.Objects.Reactor.Finite
 import ReactorModel.Objects.Reactor.Indexable
-import ReactorModel.Objects.Reactor.Practical
 import ReactorModel.Objects.Reactor.Proper
 import ReactorModel.Objects.Reactor.Theorems
 import ReactorModel.Objects.Reactor.Updatable
