src/ReactorModel/Objects/Reactor/Theorems.lean
@@ -2,8 +2,6 @@ import ReactorModel.Objects.Reactor.Theorems.Accessible
 import ReactorModel.Objects.Reactor.Theorems.Basic
 import ReactorModel.Objects.Reactor.Theorems.Extensional
 import ReactorModel.Objects.Reactor.Theorems.Finite
-import ReactorModel.Objects.Reactor.Theorems.FiniteUpdatable
 import ReactorModel.Objects.Reactor.Theorems.Indexable
-import ReactorModel.Objects.Reactor.Theorems.Practical
 import ReactorModel.Objects.Reactor.Theorems.Proper
 import ReactorModel.Objects.Reactor.Theorems.Readable
